replace old code generator by new one in Jinja

thys/Jinja/Common/Objects.thy
@@ -41,7 +41,7 @@ abbreviation
 
 definition new_Addr  :: "heap \<Rightarrow> addr option"
 where
-  "new_Addr h  \<equiv>  if \<exists>a. h a = None then Some(SOME a. h a = None) else None"
+  "new_Addr h  \<equiv>  if \<exists>a. h a = None then Some(LEAST a. h a = None) else None"
 
 definition cast_ok :: "'m prog \<Rightarrow> cname \<Rightarrow> heap \<Rightarrow> val \<Rightarrow> bool"
 where
@@ -61,7 +61,7 @@ where
 
 lemma new_Addr_SomeD:
   "new_Addr h = Some a \<Longrightarrow> h a = None"
- (*<*)by(fastsimp simp add:new_Addr_def split:if_splits intro:someI)(*>*)
+ (*<*)by(fastsimp simp add:new_Addr_def split:if_splits intro:LeastI)(*>*)
 
 lemma [simp]: "(typeof\<^bsub>h\<^esub> v = Some Boolean) = (\<exists>b. v = Bool b)"
  (*<*)by(induct v) auto(*>*)
@@ -149,5 +149,35 @@ apply(fastsimp simp:hext_def)
 done
 (*>*)
 
+text {* Code generator setup for @{term "new_Addr"} *}
+
+definition gen_new_Addr :: "heap \<Rightarrow> addr \<Rightarrow> addr option"
+where "gen_new_Addr h n \<equiv> if \<exists>a. a \<ge> n \<and> h a = None then Some(LEAST a. a \<ge> n \<and> h a = None) else None"
+
+lemma new_Addr_code_code [code]:
+  "new_Addr h = gen_new_Addr h 0"
+by(simp add: new_Addr_def gen_new_Addr_def split del: split_if cong: if_cong)
+
+lemma gen_new_Addr_code [code]:
+  "gen_new_Addr h n = (if h n = None then Some n else gen_new_Addr h (Suc n))"
+apply(simp add: gen_new_Addr_def)
+apply(rule impI)
+apply(rule conjI)
+ apply safe[1]
+  apply(fastsimp intro: Least_equality)
+ apply(rule arg_cong[where f=Least])
+ apply(rule ext)
+ apply(case_tac "n = ac")
+  apply simp
+ apply(auto)[1]
+apply clarify
+apply(subgoal_tac "a = n")
+ apply simp
+ apply(rule Least_equality)
+ apply auto[2]
+apply(rule ccontr)
+apply(erule_tac x="a" in allE)
+apply simp
+done
 
 end
