thys/Jinja/J/execute_Bigstep.thy
@@ -10,19 +10,6 @@ theory execute_Bigstep imports BigStep Examples
   "~~/src/HOL/Library/Efficient_Nat"
 begin
 
-consts_code
-  "new_Addr"
-   ("\<module>new'_addr {* 0::nat *} {* Suc *}
-               {* %x. case x of None => True | Some y => False *} {* Some *}")
-attach {*
-fun new_addr z s alloc some hp =
-  let fun nr i = if alloc (hp i) then some i else nr (s i);
-  in nr z end;
-*}
-
-  "undefined" ("(error \"undefined\")")
-
-
 inductive map_val :: "expr list \<Rightarrow> val list \<Rightarrow> bool"
 where
   Nil: "map_val [] []"
@@ -89,12 +76,11 @@ done
 
 lemma CallParamsThrow2:
   "\<lbrakk> P \<turnstile> \<langle>e,s\<^isub>0\<rangle> \<Rightarrow> \<langle>Val v,s\<^isub>1\<rangle>; P \<turnstile> \<langle>es,s\<^isub>1\<rangle> [\<Rightarrow>] \<langle>evs,s\<^isub>2\<rangle>;
-     map_val2 evs vs (throw ex # es') \<rbrakk>
+     map_val2 evs vs (throw ex # es'') \<rbrakk>
    \<Longrightarrow> P \<turnstile> \<langle>e\<bullet>M(es),s\<^isub>0\<rangle> \<Rightarrow> \<langle>throw ex,s\<^isub>2\<rangle>"
 apply(rule eval_evals.CallParamsThrow, assumption+)
 apply(simp add: map_val2_conv[symmetric])
 done
-
 
 lemma Call2:
   "\<lbrakk> P \<turnstile> \<langle>e,s\<^isub>0\<rangle> \<Rightarrow> \<langle>addr a,s\<^isub>1\<rangle>;  P \<turnstile> \<langle>ps,s\<^isub>1\<rangle> [\<Rightarrow>] \<langle>evs,(h\<^isub>2,l\<^isub>2)\<rangle>;
@@ -108,8 +94,17 @@ apply(simp add: map_val_conv[symmetric])
 apply assumption+
 done
 
+code_pred 
+  (modes: i \<Rightarrow> o \<Rightarrow> bool)
+  map_val 
+.
 
-lemmas [code_ind] =
+code_pred
+  (modes: i \<Rightarrow> o \<Rightarrow> o \<Rightarrow> bool)
+  map_val2
+.
+
+lemmas [code_pred_intro] =
  eval_evals.New eval_evals.NewFail
  eval_evals.Cast eval_evals.CastNull eval_evals.CastFail eval_evals.CastThrow
  eval_evals.Val eval_evals.Var
@@ -118,91 +113,128 @@ lemmas [code_ind] =
  eval_evals.FAcc eval_evals.FAccNull eval_evals.FAccThrow
  eval_evals.FAss eval_evals.FAssNull
  eval_evals.FAssThrow1 eval_evals.FAssThrow2
- eval_evals.CallObjThrow CallNull2 CallParamsThrow2
- Call2[simplified Method_def, OF _ _ _ _ exI,OF _ _ _ _ conjI]
+ eval_evals.CallObjThrow
+
+declare CallNull2 [code_pred_intro CallNull2]
+declare CallParamsThrow2 [code_pred_intro CallParamsThrow2]
+declare Call2 [code_pred_intro Call2]
+
+lemmas [code_pred_intro] =
  eval_evals.Block
  eval_evals.Seq eval_evals.SeqThrow
  eval_evals.CondT eval_evals.CondF eval_evals.CondThrow
  eval_evals.WhileF eval_evals.WhileT
- eval_evals.WhileCondThrow eval_evals.WhileBodyThrow
+ eval_evals.WhileCondThrow
+
+declare eval_evals.WhileBodyThrow [code_pred_intro WhileBodyThrow2]
+
+lemmas [code_pred_intro] =
  eval_evals.Throw eval_evals.ThrowNull
  eval_evals.ThrowThrow
  eval_evals.Try eval_evals.TryCatch eval_evals.TryThrow
  eval_evals.Nil eval_evals.Cons eval_evals.ConsThrow
 
+code_pred
+  (modes: i \<Rightarrow> i \<Rightarrow> i \<Rightarrow> o \<Rightarrow> o \<Rightarrow> bool as execute)
+  eval
+proof -
+  case eval
+  from eval.prems show thesis
+  proof(cases (no_simp))
+    case CallNull thus ?thesis
+      by(rule CallNull2[OF refl])(simp add: map_val_conv[symmetric])
+  next
+    case CallParamsThrow thus ?thesis
+      by(rule CallParamsThrow2[OF refl])(simp add: map_val2_conv[symmetric])
+  next
+    case Call thus ?thesis
+      by -(rule Call2[OF refl], simp_all add: map_val_conv[symmetric])
+  next
+    case WhileBodyThrow thus ?thesis by(rule WhileBodyThrow2[OF refl])
+  qed(assumption|erule (4) that[OF refl]|erule (3) that[OF refl])+
+next
+  case evals
+  from evals.prems show thesis
+    by(cases (no_simp))(assumption|erule (3) that[OF refl])+
+qed
 
-code_module Bigstep1
-contains
- test1 = "[] \<turnstile> \<langle>testExpr1,(empty,empty)\<rangle> \<Rightarrow> \<langle>_,_\<rangle>"
- test2 = "[] \<turnstile> \<langle>testExpr2,(empty,empty)\<rangle> \<Rightarrow> \<langle>_,_\<rangle>"
- test3 = "[] \<turnstile> \<langle>testExpr3,(empty,empty(''V''\<mapsto>Intg 77))\<rangle> \<Rightarrow> \<langle>_,_\<rangle>"
- test4 = "[] \<turnstile> \<langle>testExpr4,(empty,empty)\<rangle> \<Rightarrow> \<langle>_,_\<rangle>"
- test5 = "[(''Object'',('''',[],[])),(''C'',(''Object'',[(''F'',Integer)],[]))] \<turnstile> \<langle>testExpr5,(empty,empty)\<rangle> \<Rightarrow> \<langle>_,_\<rangle>"
- test6 = "[(''Object'',('''',[],[])), classI] \<turnstile> \<langle>testExpr6,(empty,empty)\<rangle> \<Rightarrow> \<langle>_,_\<rangle>"
+notation execute ("_ \<turnstile> ((1\<langle>_,/_\<rangle>) \<Rightarrow>/ \<langle>'_, '_\<rangle>)" [51,0,0] 81)
 
- V = "''V''"
- F = "''F''"
- C = "''C''"
- N = "''N''"
- L = "''L''"
+definition "test1 = [] \<turnstile> \<langle>testExpr1,(empty,empty)\<rangle> \<Rightarrow> \<langle>_,_\<rangle>"
+definition "test2 = [] \<turnstile> \<langle>testExpr2,(empty,empty)\<rangle> \<Rightarrow> \<langle>_,_\<rangle>"
+definition "test3 = [] \<turnstile> \<langle>testExpr3,(empty,empty(''V''\<mapsto>Intg 77))\<rangle> \<Rightarrow> \<langle>_,_\<rangle>"
+definition "test4 = [] \<turnstile> \<langle>testExpr4,(empty,empty)\<rangle> \<Rightarrow> \<langle>_,_\<rangle>"
+definition "test5 = [(''Object'',('''',[],[])),(''C'',(''Object'',[(''F'',Integer)],[]))] \<turnstile> \<langle>testExpr5,(empty,empty)\<rangle> \<Rightarrow> \<langle>_,_\<rangle>"
+definition "test6 = [(''Object'',('''',[],[])), classI] \<turnstile> \<langle>testExpr6,(empty,empty)\<rangle> \<Rightarrow> \<langle>_,_\<rangle>"
 
-ML {* let open Bigstep1 in if fst (DSeq.hd test1) = Val (Intg 5) then () else error "" end *}
-ML {* let open Bigstep1 in if fst (DSeq.hd test2) = Val (Intg 11) then () else error "" end *}
-ML {* let open Bigstep1 in if fst (DSeq.hd test3) = Val (Intg 83) then () else error "" end *}
-ML {*
-let open Bigstep1 in
-  if (let val (_,(h,l)) = DSeq.hd test4 in l V end) = Some (Intg 6) then () else error ""
-end
-*}
-ML {*
-let open Bigstep1 in
-  if (let val (_,(h,l)) = DSeq.hd test5
-              val Some(c,fs) = h 1
-              val Some(obj,_) = h 0
-          in (C=c,fs(F,C),[obj ,c])end)=
-    (true, Some (Intg 42), [["O","b","j","e","c","t"], ["C"]])
-    then () else error ""
-end
-*}
-ML {* let open Bigstep1 in if fst (DSeq.hd test6) = Val (Intg 160) then () else error "" end *}
-
-code_module Bigstep2
-imports Bigstep1
-contains
- test7 = "[classObject, classL] \<turnstile> \<langle>testExpr_BuildList, (empty,empty)\<rangle> \<Rightarrow> \<langle>_,_\<rangle>"
+definition "V = ''V''"
+definition "C = ''C''"
+definition "F = ''F''"
 
 ML {*
-let open Bigstep1 Bigstep2 in
-  if (let val (_,(h,_)) = DSeq.hd test7
-              val Some(_,fs1) = h 0
-              val Some(_,fs2) = h 1
-              val Some(_,fs3) = h 2
-              val Some(_,fs4) = h 3
-          in [(fs1(F,L), fs1(N,L)), (fs2(F,L), fs2(N,L)),
-              (fs3(F,L), fs3(N,L)), (fs4(F,L), fs4(N,L))] end)=
-      [(Some (Intg 1), Some (Addr 1)),
-       (Some (Intg 2), Some (Addr 2)),
-       (Some (Intg 3), Some (Addr 3)),
-       (Some (Intg 4), Some Null)] then () else error ""
-end
+  val SOME ((@{code Val} (@{code Intg} 5), _), _) = Predicate.yield @{code test1};
+  val SOME ((@{code Val} (@{code Intg} 11), _), _) = Predicate.yield @{code test2};
+  val SOME ((@{code Val} (@{code Intg} 83), _), _) = Predicate.yield @{code test3};
+
+  val SOME ((_, (_, l)), _) = Predicate.yield @{code test4};
+  val SOME (@{code Intg} 6) = l @{code V};
+
+  val SOME ((_, (h, _)), _) = Predicate.yield @{code test5};
+  val SOME (c, fs) = h 1;
+  val SOME (obj, _) = h 0;
+  val SOME (@{code Intg} i) = fs (@{code F}, @{code C});
+  if c = @{code C} andalso obj = @{code Object} andalso i = 42 
+    then () else error "";
+
+  val SOME ((@{code Val} (@{code Intg} 160), _), _) = Predicate.yield @{code test6};
 *}
 
-code_module Bigstep3
-imports Bigstep1
-contains
- test8 = "[classObject, classA] \<turnstile> \<langle>testExpr_ClassA, (empty,empty)\<rangle> \<Rightarrow> \<langle>_,_\<rangle>"
- i="''int''"
- t= "''test''"
- A="''A''"
+definition "test7 = [classObject, classL] \<turnstile> \<langle>testExpr_BuildList, (empty,empty)\<rangle> \<Rightarrow> \<langle>_,_\<rangle>"
+
+definition "L = ''L''"
+definition "N = ''N''"
 
 ML {*
-let open Bigstep1 Bigstep3 in
-  if (let val (_,(h,l)) = DSeq.hd test8
-              val Some(_,fs1) = h 0
-              val Some(_,fs2) = h 1
-          in [(fs1(i,A),fs1(t,A)), (fs2(i,A),fs2(t,A))] end)=
-      [(Some (Intg 10), Some Null), (Some (Intg 50), Some Null)] then () else error ""
-end
+  val SOME ((_, (h, _)), _) = Predicate.yield @{code test7};
+  val SOME (_, fs1) = h 0;
+  val SOME (_, fs2) = h 1;
+  val SOME (_, fs3) = h 2;
+  val SOME (_, fs4) = h 3;
+
+  val F = @{code "F"};
+  val L = @{code "L"};
+  val N = @{code "N"};
+  
+  if fs1 (F, L) = SOME (@{code Intg} 1) andalso
+     fs1 (N, L) = SOME (@{code Addr} 1) andalso
+     fs2 (F, L) = SOME (@{code Intg} 2) andalso
+     fs2 (N, L) = SOME (@{code Addr} 2) andalso
+     fs3 (F, L) = SOME (@{code Intg} 3) andalso
+     fs3 (N, L) = SOME (@{code Addr} 3) andalso
+     fs4 (F, L) = SOME (@{code Intg} 4) andalso
+     fs4 (N, L) = SOME @{code Null}
+  then () else error "";
+*}
+
+definition "test8 = [classObject, classA] \<turnstile> \<langle>testExpr_ClassA, (empty,empty)\<rangle> \<Rightarrow> \<langle>_,_\<rangle>"
+definition "i = ''int''"
+definition "t = ''test''"
+definition "A = ''A''"
+
+ML {*
+  val SOME ((_, (h, l)), _) = Predicate.yield @{code test8};
+  val SOME (_, fs1) = h 0;
+  val SOME (_, fs2) = h 1;
+
+  val i = @{code "i"};
+  val t = @{code "t"};
+  val A = @{code "A"};
+
+  if fs1 (i, A) = SOME (@{code Intg} 10) andalso 
+     fs1 (t, A) = SOME @{code Null} andalso
+     fs2 (i, A) = SOME (@{code Intg} 50) andalso 
+     fs2 (t, A) = SOME @{code Null}
+  then () else error "";
 *}
 
 end
