thys/Jinja/J/execute_WellType.thy
@@ -7,78 +7,15 @@
 header {* \isaheader{Code Generation For WellType} *}
 
 theory execute_WellType
-imports WellType Examples
+imports
+  WellType Examples
 begin
 
-(* --- WTBinOp --- *)
-lemma WTBinOpEq:
-  "\<lbrakk>P,E \<turnstile> e\<^isub>1 :: T\<^isub>1;  P,E \<turnstile> e\<^isub>2 :: T\<^isub>2; (P \<turnstile> T\<^isub>1 \<le> T\<^isub>2) \<or> (P \<turnstile> T\<^isub>2 \<le> T\<^isub>1)\<rbrakk> \<Longrightarrow> P,E \<turnstile> e\<^isub>1 \<guillemotleft>Eq\<guillemotright> e\<^isub>2 :: Boolean"
-by (simp add: WT_WTs.WTBinOpEq)
-
-lemma WTBinOpAdd:
-  "\<lbrakk>P,E \<turnstile> e\<^isub>1 :: T\<^isub>1;  P,E \<turnstile> e\<^isub>2 :: T\<^isub>2; T\<^isub>1 = Integer; T\<^isub>2 = Integer\<rbrakk> \<Longrightarrow> P,E \<turnstile> e\<^isub>1 \<guillemotleft>Add\<guillemotright> e\<^isub>2 :: Integer"
-by (simp add: WTBinOpAdd)
-
-(* Could not finish proof \<Rightarrow> WT_WTs.WTCond replaced with new intros WT_WTs.WTCond1 and WT_WTs.WTCond2 *)
-(* --- WTCond --- *)
-(*
-lemma TRSubclsWf:
-  "wf ( (subcls1 P)\<^sup>* )"
-sorry
-
-lemma TRSubclsLe:
-  assumes noteq: "C \<noteq> D" and subcls: "P \<turnstile> C \<preceq>\<^sup>* D"
-  shows "\<not> P \<turnstile> D \<preceq>\<^sup>* C"
-proof (cases "C = Object")
-  case True
-  note Obj=True
-  thus ?thesis
-  proof (cases "D = Object")
-    case True
-    with noteq Obj show ?thesis by simp
-  next
-    case False
-    with subcls Obj show ?thesis by simp
-  qed
-next
-  case False
-  note Obj=False
-  with noteq subcls show ?thesis
-  proof (cases "D = Object")
-    case True
-    with noteq show ?thesis by simp
-  next
-    case False
-    with noteq subcls Obj show ?thesis by (rule_tac wf_not_sym, simp add: TRSubclsWf)
-  qed
-qed
-
-lemma TRSubclsEq:
-  assumes subcls1: "P \<turnstile> C \<preceq>\<^sup>* D" and subcls2: "P \<turnstile> D \<preceq>\<^sup>* C"
-  shows "C = D"
-proof (cases "C = Object")
-  case True
-  with subcls1 have "D = Object" by simp
-  thus ?thesis by simp
-next
-  case False
-  with subcls2 have Obj: "D \<noteq> Object" by auto
-  with False subcls1 subcls2 show ?thesis
-  proof (cases "C = D")
-    case True thus ?thesis by simp
-  next
-    case False with Obj subcls1 subcls2 show ?thesis by (simp add: TRSubclsLe)
-  qed
-qed
-
-lemma TRWidenEq:
-  "\<lbrakk> P \<turnstile> T\<^isub>1 \<le> T\<^isub>2; P \<turnstile> T\<^isub>2 \<le> T\<^isub>1\<rbrakk> \<Longrightarrow> T\<^isub>1 = T\<^isub>2"
-by (cases T\<^isub>1,auto, cases T\<^isub>2,auto simp add:TRSubclsEq)
-*)
+(* Replace WT_WTs.WTCond with new intros WT_WTs.WTCond1 and WT_WTs.WTCond2 *)
 
 lemma WTCond1:
   "\<lbrakk>P,E \<turnstile> e :: Boolean;  P,E \<turnstile> e\<^isub>1::T\<^isub>1;  P,E \<turnstile> e\<^isub>2::T\<^isub>2; P \<turnstile> T\<^isub>1 \<le> T\<^isub>2;
-    P \<turnstile> T\<^isub>2 \<le> T\<^isub>1 \<longrightarrow> T\<^isub>1 = T\<^isub>2 \<rbrakk> \<Longrightarrow> P,E \<turnstile> if (e) e\<^isub>1 else e\<^isub>2 :: T\<^isub>2"
+    P \<turnstile> T\<^isub>2 \<le> T\<^isub>1 \<longrightarrow> T\<^isub>2 = T\<^isub>1 \<rbrakk> \<Longrightarrow> P,E \<turnstile> if (e) e\<^isub>1 else e\<^isub>2 :: T\<^isub>2"
 by (fastsimp)
 
 lemma WTCond2:
@@ -86,64 +23,96 @@ lemma WTCond2:
     P \<turnstile> T\<^isub>1 \<le> T\<^isub>2 \<longrightarrow> T\<^isub>1 = T\<^isub>2 \<rbrakk> \<Longrightarrow> P,E \<turnstile> if (e) e\<^isub>1 else e\<^isub>2 :: T\<^isub>1"
 by (fastsimp)
 
-lemmas [code_ind] =
+lemmas [code_pred_intro] =
   WT_WTs.WTNew
   WT_WTs.WTCast
   WT_WTs.WTVal
   WT_WTs.WTVar
-         WTBinOpEq WTBinOpAdd (*WT.WT_WTs.WTBinOp*)
+  WT_WTs.WTBinOpEq
+  WT_WTs.WTBinOpAdd
   WT_WTs.WTLAss
-  WT_WTs.WTFAcc[unfolded sees_field_def, OF _ exI, OF _ conjI]
-  WT_WTs.WTFAss[unfolded sees_field_def, OF _ exI, OF _ conjI]
-  WT_WTs.WTCall[unfolded Method_def, OF _ exI, OF _ conjI]
+  WT_WTs.WTFAcc
+  WT_WTs.WTFAss
+  WT_WTs.WTCall
   WT_WTs.WTBlock
   WT_WTs.WTSeq
-  WTCond1
-  WTCond2
+
+declare
+  WTCond1 [code_pred_intro WTCond1]
+  WTCond2 [code_pred_intro WTCond2]
+
+lemmas [code_pred_intro] =
   WT_WTs.WTWhile
   WT_WTs.WTThrow
   WT_WTs.WTTry
   WT_WTs.WTNil
   WT_WTs.WTCons
 
+code_pred
+  (modes: i \<Rightarrow> i \<Rightarrow> i \<Rightarrow> i \<Rightarrow> bool as type_check, i \<Rightarrow> i \<Rightarrow> i \<Rightarrow> o \<Rightarrow> bool as infer_type)
+  WT
+proof -
+  case WT
+  from WT.prems show thesis
+  proof(cases (no_simp))
+    case (WTCond E e e1 T1 e2 T2 T)
+    from `x \<turnstile> T1 \<le> T2 \<or> x \<turnstile> T2 \<le> T1` show thesis
+    proof
+      assume "x \<turnstile> T1 \<le> T2"
+      with `x \<turnstile> T1 \<le> T2 \<longrightarrow> T = T2` have "T = T2" ..
+      from `xa = E` `xb = if (e) e1 else e2` `xc = T` `x,E \<turnstile> e :: Boolean` 
+        `x,E \<turnstile> e1 :: T1` `x,E \<turnstile> e2 :: T2` `x \<turnstile> T1 \<le> T2` `x \<turnstile> T2 \<le> T1 \<longrightarrow> T = T1`
+      show ?thesis unfolding `T = T2` by(rule WTCond1[OF refl])
+    next
+      assume "x \<turnstile> T2 \<le> T1"
+      with `x \<turnstile> T2 \<le> T1 \<longrightarrow> T = T1` have "T = T1" ..
+      from `xa = E` `xb = if (e) e1 else e2` `xc = T` `x,E \<turnstile> e :: Boolean` 
+        `x,E \<turnstile> e1 :: T1` `x,E \<turnstile> e2 :: T2` `x \<turnstile> T2 \<le> T1` `x \<turnstile> T1 \<le> T2 \<longrightarrow> T = T2`
+      show ?thesis unfolding `T = T1` by(rule WTCond2[OF refl])
+    qed
+  qed(assumption|erule (2) that[OF refl])+
+next
+  case WTs
+  from WTs.prems show thesis
+    by(cases (no_simp))(assumption|erule (2) that[OF refl])+
+qed
 
-code_module WellType1
-contains
-  test1 = "[], empty  \<turnstile> testExpr1 :: _"
-  test2 = "[], empty  \<turnstile> testExpr2 :: _"
-  test3 = "[], empty(''V'' \<mapsto> Integer)  \<turnstile> testExpr3 :: _"
-  test4 = "[], empty(''V'' \<mapsto> Integer)  \<turnstile> testExpr4 :: _"
-  test5 = "[classObject, (''C'',(''Object'',[(''F'',Integer)],[]))], empty  \<turnstile> testExpr5 :: _"
-  test6 = "[classObject, classI], empty  \<turnstile> testExpr6 :: _"
+notation infer_type ("_,_ \<turnstile> _ :: '_" [51,51,51]100)
 
-ML {* let open WellType1 in if DSeq.hd test1 = Integer then () else error "" end *}
-ML {* let open WellType1 in if DSeq.hd test2 = Integer then () else error "" end *}
-ML {* let open WellType1 in if DSeq.hd test3 = Integer then () else error "" end *}
-ML {* let open WellType1 in if DSeq.hd test4 = Void then () else error "" end *}
-ML {* let open WellType1 in if DSeq.hd test5 = Void then () else error "" end *}
-ML {* let open WellType1 in if DSeq.hd test6 = Integer then () else error "" end *}
+definition test1 where "test1 = [],empty \<turnstile> testExpr1 :: _"
+definition test2 where "test2 = [], empty  \<turnstile> testExpr2 :: _"
+definition test3 where "test3 = [], empty(''V'' \<mapsto> Integer)  \<turnstile> testExpr3 :: _"
+definition test4 where "test4 = [], empty(''V'' \<mapsto> Integer)  \<turnstile> testExpr4 :: _"
+definition test5 where "test5 = [classObject, (''C'',(''Object'',[(''F'',Integer)],[]))], empty  \<turnstile> testExpr5 :: _"
+definition test6 where "test6 = [classObject, classI], empty  \<turnstile> testExpr6 :: _"
 
-code_module WellType2
-imports WellType1
-contains
-  testmb_isNull     = "[classObject, classA], empty([this] [\<mapsto>] [Class ''A'']) \<turnstile> mb_isNull :: _"
-  testmb_add        = "[classObject, classA], empty([this,''i''] [\<mapsto>] [Class ''A'',Integer]) \<turnstile> mb_add :: _"
-  testmb_mult_cond  = "[classObject, classA], empty([this,''j''] [\<mapsto>] [Class ''A'',Integer]) \<turnstile> mb_mult_cond :: _"
-  testmb_mult_block = "[classObject, classA], empty([this,''i'',''j'',''temp''] [\<mapsto>] [Class ''A'',Integer,Integer,Integer]) \<turnstile> mb_mult_block :: _"
-  testmb_mult       = "[classObject, classA], empty([this,''i'',''j''] [\<mapsto>] [Class ''A'',Integer,Integer]) \<turnstile> mb_mult :: _"
+ML {*
+  val SOME(@{code Integer}, _) = Predicate.yield @{code test1};
+  val SOME(@{code Integer}, _) = Predicate.yield @{code test2};
+  val SOME(@{code Integer}, _) = Predicate.yield @{code test3};
+  val SOME(@{code Void}, _) = Predicate.yield @{code test4};
+  val SOME(@{code Void}, _) = Predicate.yield @{code test5};
+  val SOME(@{code Integer}, _) = Predicate.yield @{code test6};
+*}
 
-ML {* let open WellType1 WellType2 in if DSeq.hd testmb_isNull = Boolean then () else error "" end *}
-ML {* let open WellType1 WellType2 in if DSeq.hd testmb_add = Integer then () else error "" end *}
-ML {* let open WellType1 WellType2 in if DSeq.hd testmb_mult_cond = Boolean then () else error "" end *}
-ML {* let open WellType1 WellType2 in if DSeq.hd testmb_mult_block = Void then () else error "" end *}
-ML {* let open WellType1 WellType2 in if DSeq.hd testmb_mult = Integer then () else error "" end *}
+definition testmb_isNull where "testmb_isNull = [classObject, classA], empty([this] [\<mapsto>] [Class ''A'']) \<turnstile> mb_isNull :: _"
+definition testmb_add where "testmb_add = [classObject, classA], empty([this,''i''] [\<mapsto>] [Class ''A'',Integer]) \<turnstile> mb_add :: _"
+definition testmb_mult_cond where "testmb_mult_cond = [classObject, classA], empty([this,''j''] [\<mapsto>] [Class ''A'',Integer]) \<turnstile> mb_mult_cond :: _"
+definition testmb_mult_block where "testmb_mult_block = [classObject, classA], empty([this,''i'',''j'',''temp''] [\<mapsto>] [Class ''A'',Integer,Integer,Integer]) \<turnstile> mb_mult_block :: _"
+definition testmb_mult where "testmb_mult = [classObject, classA], empty([this,''i'',''j''] [\<mapsto>] [Class ''A'',Integer,Integer]) \<turnstile> mb_mult :: _"
 
-code_module WellType3
-imports WellType1
-contains
-  test = "[classObject, classA], empty \<turnstile> testExpr_ClassA :: _"
+ML {*
+  val SOME(@{code Boolean}, _) = Predicate.yield @{code testmb_isNull};
+  val SOME(@{code Integer}, _) = Predicate.yield @{code testmb_add};
+  val SOME(@{code Boolean}, _) = Predicate.yield @{code testmb_mult_cond};
+  val SOME(@{code Void}, _) = Predicate.yield @{code testmb_mult_block};
+  val SOME(@{code Integer}, _) = Predicate.yield @{code testmb_mult};
+*}
 
-ML {* let open WellType1 WellType3 in if DSeq.hd test = Integer then () else error "" end *}
+definition test where "test = [classObject, classA], empty \<turnstile> testExpr_ClassA :: _"
 
+ML {*
+  val SOME(@{code Integer}, _) = Predicate.yield @{code test};
+*}
 
 end
